examples/Sek/PArray_proof.v
@@ -48,7 +48,7 @@ Ltac set_prove_setup use_classic ::=
 
 
 
-Hint Extern 1 (dom _ \c dom _) => rew_map; set_prove.
+Hint Extern 1 (dom _ \c _) => rew_map; set_prove.
 (*
 Hint Extern 1 (_ \in dom _) => rew_map; saturate_indom; set_prove.
 *)
@@ -103,6 +103,12 @@ Ltac set_prove2 := (* set_prove fails sometimes *)
 	set_prove_setup false; intuition.
 
 
+Ltac set_specialize_hyps A x ::=
+	repeat match goal with H: forall _:A, _ |- _ =>
+		specializes H x
+	end.
+
+
 Tactic Notation "tryifalse" :=
 	try solve [intros; false].
 
@@ -126,7 +132,6 @@ Inductive Desc A :=
   |	Desc_Base : list A -> Desc A 
   |	Desc_Diff : loc -> int -> A -> Desc A.
 
-#[global]
 Instance Desc_inhab A : Inhab A -> Inhab (Desc A).
 Proof using. intros. apply (Inhab_of_val (Desc_Base nil)). Qed.
 
@@ -177,21 +182,52 @@ Proof using. intros. intros ? ?. apply haffine_PArray_Desc. Qed.
 Hint Resolve haffine_PArray_Desc haffine_repr_PArray_Desc : haffine.
 
 
-Definition PArray A {IA: Inhab A} {EA: Enc A} (D: Desc A) (pa: parray_ A) : hprop :=
-	\exists d, pa ~~~> `{ data' := d } \* d ~> PArray_Desc D.
+Record PArray_Rec A : Type := {
+	desc : Desc A;
+	maxdist : int }.
 
-Lemma PArray_eq : forall A (IA: Inhab A) (EA: Enc A) (pa: parray_ A) (D: Desc A),
-	pa ~> PArray D =
-	\exists d, pa ~~~> `{ data' := d } \* d ~> PArray_Desc D.
+Instance PArray_Rec_inhab A : Inhab A -> Inhab (PArray_Rec A).
+Proof using. intros. apply (Inhab_of_val {| desc := arbitrary; maxdist := 0 |}). Qed.
+
+Hint Resolve PArray_Rec_inhab.
+
+Lemma PArray_Rec_eq : forall A (rec: PArray_Rec A),
+	rec = {| desc := desc rec; maxdist := maxdist rec |}.
+Proof using. intros. destruct* rec. Qed.
+
+Lemma PArray_Rec_eq_desc : forall A (D: Desc A) (md: int),
+	desc {| desc := D; maxdist := md |} = D.
 Proof using. auto. Qed.
 
-Lemma PArray_Base_close : forall A (IA: Inhab A) (EA: Enc A) (pa: parray_ A) (a: array A) (L: list A),
-	pa ~~~> `{ data' := PArray_Base a } \* a ~> Array L ==> pa ~> PArray (Desc_Base L).
-Proof using. intros. xchange* <- PArray_Desc_eq_Base. xchange* <- PArray_eq. Qed.
+Lemma PArray_Rec_eq_maxdist : forall A (D: Desc A) (md: int),
+	maxdist {| desc := D; maxdist := md |} = md.
+Proof using. auto. Qed.
 
-Lemma PArray_Diff_close : forall A (IA: Inhab A) (EA: Enc A) (pa: parray_ A) q i x,
-	pa ~~~> `{ data' := PArray_Diff q i x } ==> pa ~> PArray (Desc_Diff q i x).
-Proof using. intros. xchange* <- PArray_Desc_eq_Diff q i x. xchange* <- PArray_eq. Qed.
+Hint Rewrite PArray_Rec_eq_desc PArray_Rec_eq_maxdist.
+
+Definition PArray A {IA: Inhab A} {EA: Enc A} (rec: PArray_Rec A) (pa: parray_ A) : hprop :=
+	\exists d, pa ~~~> `{ data' := d ; maxdist' := maxdist rec } \* d ~> PArray_Desc (desc rec).
+
+Lemma PArray_eq : forall A (IA: Inhab A) (EA: Enc A) (pa: parray_ A) (rec: PArray_Rec A),
+	pa ~> PArray rec =
+	\exists d, pa ~~~> `{ data' := d ; maxdist' := maxdist rec } \* d ~> PArray_Desc (desc rec).
+Proof using. auto. Qed.
+
+Lemma PArray_Base_close : forall A (IA: Inhab A) (EA: Enc A) (pa: parray_ A) (a: array A) (md: int) (L: list A),
+	pa ~~~> `{ data' := PArray_Base a; maxdist' := md } \* a ~> Array L ==>
+	pa ~> PArray {| desc := Desc_Base L; maxdist := md |}.
+Proof using.
+	intros. xchange* <- PArray_Desc_eq_Base.
+	xchange* <- PArray_eq {| desc := Desc_Base L; maxdist := md |}.
+Qed.
+
+Lemma PArray_Diff_close : forall A (IA: Inhab A) (EA: Enc A) (pa: parray_ A) (md: int) q i x,
+	pa ~~~> `{ data' := PArray_Diff q i x; maxdist' := md } ==>
+	pa ~> PArray {| desc := Desc_Diff q i x; maxdist := md |}.
+Proof using.
+	intros. xchange* <- PArray_Desc_eq_Diff q i x.
+	xchange* <- PArray_eq {| desc := Desc_Diff q i x; maxdist := md |}.
+Qed.
 
 Hint Extern 1 (RegisterOpen PArray) => Provide PArray_eq.
 
@@ -205,8 +241,8 @@ Qed.
 
 Hint Resolve Heapdata_PArray.
 
-Lemma haffine_PArray : forall A (IA: Inhab A) (EA: Enc A) (D: Desc A) (pa: parray_ A),
-    haffine (pa ~> PArray D).
+Lemma haffine_PArray : forall A (IA: Inhab A) (EA: Enc A) (rec: PArray_Rec A) (pa: parray_ A),
+    haffine (pa ~> PArray rec).
 Proof using. intros. rewrite PArray_eq. xaffine. Qed.
 
 Lemma haffine_repr_PArray : forall A (IA: Inhab A) (EA: Enc A),
@@ -216,14 +252,14 @@ Proof using. intros. intros ? ?. apply haffine_PArray. Qed.
 Hint Resolve haffine_PArray haffine_repr_PArray : haffine.
 
 
-Notation "'Memory' A" := (map (parray_ A) (Desc A)) (at level 69).
+Notation "'Memory' A" := (map (parray_ A) (PArray_Rec A)) (at level 69).
 
 Lemma Memory_eq_inv_Base : forall A (IA: Inhab A) (EA: Enc A) (M: Memory A) (pa: parray_ A) (L L': list A),
-	M[pa] = Desc_Base L -> M[pa] = Desc_Base L' -> L = L'.
+	desc (M[pa]) = Desc_Base L -> desc (M[pa]) = Desc_Base L' -> L = L'.
 Proof using. introv EA E E'. rewrites* E in E'. inverts* E'. Qed.
 
 Lemma Memory_eq_inv_Desc : forall A (IA: Inhab A) (EA: Enc A) (M: Memory A) (pa: parray_ A) q i x r j y,
-	M[pa] = Desc_Diff q i x -> M[pa] = Desc_Diff r j y -> (q, i, x) = (r, j, y).
+	desc (M[pa]) = Desc_Diff q i x -> desc (M[pa]) = Desc_Diff r j y -> (q, i, x) = (r, j, y).
 Proof using. introv EA E E'. rewrites* E in E'. inverts* E'. Qed.
 
 Hint Resolve Memory_eq_inv_Base Memory_eq_inv_Desc.
@@ -231,14 +267,16 @@ Hint Resolve Memory_eq_inv_Base Memory_eq_inv_Desc.
 Inductive IsPArray A {IA: Inhab A} {EA: Enc A} (M: Memory A) : list A -> parray_ A -> Prop :=
 	|	IsPArray_Base : forall pa L,
 			pa \indom M ->
-			M[pa] = Desc_Base L ->
+			desc (M[pa]) = Desc_Base L ->
+			maxdist (M[pa]) <= length L ->
 			IsPArray M L pa
 	|	IsPArray_Diff : forall pa' pa i x L' L,
 			pa \indom M ->
-			M[pa] = Desc_Diff pa' i x ->
+			desc (M[pa]) = Desc_Diff pa' i x ->
 			IsPArray M L' pa' ->
 			index L' i ->
 			L = L'[i := x] ->
+			maxdist (M[pa]) < maxdist (M[pa']) ->
 			IsPArray M L pa.
 
 Lemma IsPArray_inv_indom : forall A (IA: Inhab A) (EA: Enc A) (M: Memory A) (pa: parray_ A) (L: list A),
@@ -271,19 +309,32 @@ Proof using. introv Rpa Rpa' HL <-. forwards*: IsPArray_inv_eq. Qed.
 
 Hint Resolve IsPArray_inv_neq.
 
+Lemma IsPArray_inv_maxdist : forall A (IA: Inhab A) (EA: Enc A) (M: Memory A) (pa: parray_ A) (L: list A),
+	IsPArray M L pa ->
+	maxdist (M[pa]) <= length L.
+Proof using.
+	introv Rpa. induction Rpa as [| q pa i x L' L Hpa E Rq IH Hi EL Hdist]; auto.
+	forwards* Elen: length_update L' i x.
+	rewrites* <- EL in Elen. rewrites* <- Elen in IH. transitivity (maxdist M[q]); auto.
+Qed.
+
+Hint Resolve IsPArray_inv_maxdist.
+
 Section IsPArray_sized.
 
 Inductive IsPArray_sized A {IA: Inhab A} {EA: Enc A} (M: Memory A) : list A -> parray_ A -> nat -> Prop :=
 	|	IsPArray_Base_sized : forall pa L,
 			pa \indom M ->
-			M[pa] = Desc_Base L ->
+			desc (M[pa]) = Desc_Base L ->
+			maxdist (M[pa]) <= length L ->
 			IsPArray_sized M L pa 0
 	|	IsPArray_Diff_sized : forall pa' pa i x L' L n,
 			pa \indom M ->
-			M[pa] = Desc_Diff pa' i x ->
+			desc (M[pa]) = Desc_Diff pa' i x ->
 			IsPArray_sized M L' pa' n ->
 			index L' i ->
 			L = L'[i := x] ->
+			maxdist (M[pa]) < maxdist (M[pa']) ->
 			IsPArray_sized M L pa (S n).
 
 Hint Constructors IsPArray IsPArray_sized.
@@ -320,25 +371,35 @@ Hint Resolve indom_of_union_single_neq.
 Hint Rewrite dom_of_union_single_eq : rew_set.
 
 
-Definition Points_into {A} {IA: Inhab A} {EA: Enc A} (R: set (parray_ A)) (D: Desc A) : Prop :=
-	match D with
+Definition Points_into {A} {IA: Inhab A} {EA: Enc A} (R: set (parray_ A)) (rec: PArray_Rec A) : Prop :=
+	match desc rec with
 	|	Desc_Base _ => True
 	|	Desc_Diff q _ _ => q \in R
 	end.
 
-Lemma Points_into_Base : forall A (IA: Inhab A) (EA: Enc A) (R: set (parray_ A)) (L: list A),
-	Points_into R (Desc_Base L).
-Proof using. unfold Points_into. auto. Qed.
+Lemma Points_into_Base : forall A (IA: Inhab A) (EA: Enc A) (R: set (parray_ A)) (L: list A) (md: int),
+	Points_into R {| desc := Desc_Base L; maxdist := md |}.
+Proof using. unfold Points_into. intros. simpl. auto. Qed.
 
-Lemma Points_into_eq_Diff : forall A (IA: Inhab A) (EA: Enc A) (R: set (parray_ A)) q i x,
-	Points_into R (Desc_Diff q i x) = q \in R.
-Proof using. unfold Points_into. auto. Qed.
+Lemma Points_into_of_eq_Base : forall A (IA: Inhab A) (EA: Enc A) (R: set (parray_ A)) (rec: PArray_Rec A) (L: list A),
+	desc rec = Desc_Base L ->
+	Points_into R rec.
+Proof using. unfold Points_into. introv IA EA ->. auto. Qed.
 
-Lemma Points_into_subset : forall A (IA: Inhab A) (EA: Enc A) (R R': set (parray_ A)) (D: Desc A),
-	R \c R' -> Points_into R D -> Points_into R' D.
-Proof using. introv HR. destruct* D. applys* HR. Qed.
+Lemma Points_into_eq_Diff : forall A (IA: Inhab A) (EA: Enc A) (R: set (parray_ A)) q i x (md: int),
+	Points_into R {| desc := Desc_Diff q i x; maxdist := md |} = q \in R.
+Proof using. unfold Points_into. intros. simpl. auto. Qed.
 
-Hint Resolve Points_into_Base Points_into_eq_Diff Points_into_subset.
+Lemma Points_into_eq_of_eq_Diff : forall A (IA: Inhab A) (EA: Enc A) (R: set (parray_ A)) (rec: PArray_Rec A) q i x,
+	desc rec = Desc_Diff q i x ->
+	Points_into R rec = q \in R.
+Proof using. unfold Points_into. introv IA EA ->. auto. Qed.
+
+Lemma Points_into_subset : forall A (IA: Inhab A) (EA: Enc A) (R R': set (parray_ A)) (rec: PArray_Rec A),
+	R \c R' -> Points_into R rec -> Points_into R' rec.
+Proof using. introv HR. lets* [[L | q i x] md]: rec. applys* HR. Qed.
+
+Hint Resolve Points_into_Base Points_into_of_eq_Base Points_into_eq_Diff Points_into_eq_of_eq_Diff Points_into_subset.
 
 
 Definition Points_into_forall A {IA: Inhab A} {EA: Enc A} (R: set (parray_ A)) (M: Memory A) : Prop :=
@@ -353,10 +414,10 @@ Lemma Points_into_forall_subset : forall A (IA: Inhab A) (EA: Enc A) (R R': set 
 Proof using. introv HR. unfold Points_into_forall. intros H p Hp. applys* Points_into_subset. Qed.
 
 Lemma Points_into_forall_update :
-	forall A (IA: Inhab A) (EA: Enc A) (R: set (parray_ A)) (M: Memory A) (pa: parray_ A) (D: Desc A),
+	forall A (IA: Inhab A) (EA: Enc A) (R: set (parray_ A)) (M: Memory A) (pa: parray_ A) (rec: PArray_Rec A),
 		Points_into_forall R M ->
-		Points_into R D ->
-		Points_into_forall R (M[pa := D]).
+		Points_into R rec ->
+		Points_into_forall R (M[pa := rec]).
 Proof using.
 	introv Hforall H. rewrite Points_into_forall_eq. intros p Hp.
 	rew_map in *. rewrites* read_update.
@@ -406,25 +467,26 @@ Lemma Shared_inv_focus : forall A (IA: Inhab A) (EA: Enc A) (M: Memory A) (pa: p
 	Shared M ==>
 		\[Inv M] \*
 		pa ~> PArray (M[pa]) \*
-		\forall D,
-			pa ~> PArray D \-*
-			\[Points_into (dom M) D] \-*
-			Shared (M[pa := D]).
+		\forall rec,
+			pa ~> PArray rec \-*
+			\[Points_into (dom M) rec] \-*
+			Shared (M[pa := rec]).
 Proof using.
 	intros. unfold Shared. xchange* Group_focus pa.
 	forwards* Dpa: IsPArray_inv_indom.
-	intros I. xsimpl*; intros D.
+	intros I. xsimpl*; intros rec.
 	{ constructors*.
 		{ rewrites* Points_into_forall_eq. intros p Hdom.
 			rew_map in *. rewrites* <- dom_of_union_single_eq in *.
 			rewrites* read_update. case_if*.
 			applys* Inv_closure I. } }
-	{ xchange* hforall_specialize D. }
+	{ xchange* hforall_specialize rec. }
 Qed.
 
-Lemma Shared_add_fresh_Base : forall A (IA: Inhab A) (EA: Enc A) (M: Memory A) (pa: parray_ A) (L: list A),
-  pa ~> PArray (Desc_Base L) \* Shared M 
-  ==> Shared (M[pa := Desc_Base L]) \* \[pa \notindom M].
+Lemma Shared_add_fresh_Base : forall A (IA: Inhab A) (EA: Enc A) (M: Memory A) (pa: parray_ A) (rec: PArray_Rec A) (L: list A),
+  desc rec = Desc_Base L ->
+	pa ~> PArray rec \* Shared M 
+  ==> Shared (M[pa := rec]) \* \[pa \notindom M].
 Proof using.
 	intros. unfold Shared. xchanges* Group_add_fresh.
 	intros I Hpa. constructors*.
@@ -447,56 +509,67 @@ Lemma Extend_trans : forall A (IA: Inhab A) (EA: Enc A) (M1 M2 M3: Memory A),
 	Extend M1 M2 -> Extend M2 M3 -> Extend M1 M3.
 Proof using.
 	unfold Extend. introv [Hdom1 Harr1] [Hdom2 Harr2]. split*.
-Unshelve. apply nil. apply nil. (* Un peu débile *) Qed.
+Qed.
 
-Lemma Extend_add_fresh : forall A (IA: Inhab A) (EA: Enc A) (M: Memory A) (pa: parray_ A) (D: Desc A),
+Lemma Extend_add_fresh : forall A (IA: Inhab A) (EA: Enc A) (M: Memory A) (pa: parray_ A) (rec: PArray_Rec A),
 	~(pa \indom M) ->
-	Extend M (M[pa := D]).
+	Extend M (M[pa := rec]).
 Proof using.
 	introv H. unfold Extend. split*.
 	intros L p Rp. induction Rp.
-	{ applys* IsPArray_Base. rew_map*. }
-	{ applys* IsPArray_Diff. rew_map*. }
+	{ applys* IsPArray_Base; rew_map*. }
+	{ applys* IsPArray_Diff; rew_map*. forwards*: IsPArray_inv_indom M pa'. }
 Qed.
 
-Lemma Extend_update_Base : forall A (IA: Inhab A) (EA: Enc A) (M: Memory A) (pa: parray_ A) (L: list A),
+Lemma Extend_update_Base : forall A (IA: Inhab A) (EA: Enc A) (M: Memory A) (pa: parray_ A) (rec: PArray_Rec A) (L: list A),
 	IsPArray M L pa ->
-	Extend M (M[pa := Desc_Base L]).
+	desc rec = Desc_Base L ->
+	maxdist (M[pa]) <= maxdist rec ->
+	maxdist rec <= length L ->
+	Extend M (M[pa := rec]).
 Proof using.
-	introv Rpa. unfold Extend.
+	introv Rpa HD Hlb Hub. unfold Extend.
 	split*. intros Lq q Rq. induction Rq as [q Lq Hq E | p q i x Lp Lq Hq E Rp IH Hi EL].
-	{ applys* IsPArray_Base. rewrites* read_update. case_if*.
-		rewrite <- C in *.
-		inverts* Rpa as; tryifalse. intros Hpa E'. rewrites* E in E'. }
+	{ applys* IsPArray_Base; rewrites* read_update; case_if*;
+		rewrite <- C in *;
+		inverts* Rpa as; tryifalse; intros Hpa E' Hdist'; rewrites* E in E'.
+		{ rewrites* HD. }
+		{ inverts* E'. } }
 	{ tests : (q = pa).
-		{	applys* IsPArray_Base. rew_map*.
-			forwards* Rpa': IsPArray_Diff p pa.
-			fequals*. }
-		{ applys* IsPArray_Diff. rew_map*. } }
+		{	applys* IsPArray_Base; rew_map*;
+			forwards* Rpa': IsPArray_Diff p pa; forwards* EL': IsPArray_inv_eq M pa (Lp[i := x]) L.
+			rewrites* <- EL in EL'. rewrites* EL'. auto. }
+		{ applys* IsPArray_Diff.
+			{ rew_map*. }
+			{ rewrites* (>> read_update p). case_if*; rew_map*. rewrite <- C0 in *.
+				(* Clairement vrai, mais math ne fonctionne pas. *)skip. } } }
 Qed.
 
-Lemma Extend_update_Diff : forall A (IA: Inhab A) (EA: Enc A) (M: Memory A) (pa: parray_ A) (L: list A) q i x,
+Lemma Extend_update_Diff : forall A (IA: Inhab A) (EA: Enc A) (M: Memory A) (pa: parray_ A) (rec: PArray_Rec A) (L: list A) q i x,
 	index L i ->
 	IsPArray M (L[i := x]) pa ->
-	q \indom M ->
 	q <> pa ->
-	M[q] = Desc_Base L ->
-	Extend M (M[pa := Desc_Diff q i x]).
+	desc (M[q]) = Desc_Base L ->
+	IsPArray M L q ->
+	desc rec = Desc_Diff q i x ->
+	maxdist (M[pa]) <= maxdist rec ->
+	maxdist rec < maxdist (M[q]) ->
+	Extend M (M[pa := rec]).
 Proof using.
-	introv Hi Rpa Hq Hdiff Mq. unfold Extend.
+	introv Hi Rpa Hdiff Mq Rq HD Hlb Hub. unfold Extend.
 	split*. intros Lp p Rp. induction Rp as [p Lp Hp E | r p j y Lr Lp Hp E Rr IH Hj EL].
 	{	tests : (p = pa).
-		{ applys* IsPArray_Diff q i x L.
-			{ rew_map*. }
-			{ applys* IsPArray_Base. rew_map*. }
+		{ applys* IsPArray_Diff q i x L; rew_map*.
+			{ applys* IsPArray_Base; rew_map*. rew_set. forwards*: IsPArray_inv_indom. }
 			{ forwards*: IsPArray_Base. } }
-		{ applys* IsPArray_Base. rew_map*. } }
+		{ applys* IsPArray_Base; rew_map*. } }
 	{ tests : (p = pa).
-		{ applys* IsPArray_Diff q i x L.
-			{ rew_map*. }
-			{ applys* IsPArray_Base. rew_map*. }
+		{ applys* IsPArray_Diff q i x L; rew_map*.
+			{ applys* IsPArray_Base; rew_map*. rew_set. forwards*: IsPArray_inv_indom M q. }
 			{ forwards*: IsPArray_Diff r pa. } }
-		{ applys* IsPArray_Diff. rew_map*. } }
+		{ applys* IsPArray_Diff.
+			{ rew_map*. }
+			{ rewrites* (>> read_update r). case_if*; rew_map*. rewrite <- C0 in *. (* Idem. *) skip. } } }
 Qed.
 
 Hint Resolve IsPArray_Extend Extend_trans Extend_add_fresh Extend_update_Base Extend_update_Diff.
@@ -517,12 +590,13 @@ Lemma parray_create_spec : forall A (IA: Inhab A) (EA: Enc A) (M: Memory A) (sz:
 		PRE \[]
 		POST (fun M' pa => \[IsPArray M' (make sz d) pa]).
 Proof using.
-	introv Hsz. xcf*. simpl. xpay_skip.
+	introv Hsz. xcf*. simpl. xpay_fake.
 	xapp*. intros a L ->.
 	xapp*. intros pa.
 	xchange* PArray_Base_close.
-	xchanges* Shared_add_fresh_Base; intros Hpa.
-	apply* IsPArray_Base. rew_map*.
+	xchanges* Shared_add_fresh_Base (make sz d). intros Hpa.
+	apply* IsPArray_Base; rew_map*.
+	simpl. auto.
 Qed.
 
 Hint Extern 1 (RegisterSpec parray_create) => Provide parray_create_spec.
@@ -542,27 +616,25 @@ Lemma parray_base_copy_spec : forall A (IA: Inhab A) (EA: Enc A) (M: Memory A) (
 Proof using.
 	introv Rpa. lets (n & Rpas): IsPArray_sized_of_unsized Rpa.
 	gen pa L. induction_wf IH: wf_lt n.
-	introv Rpa. xcf*. xpay_skip.
+	introv Rpa. xcf*. xpay_fake.
 	xchange* Shared_inv_focus. intros I.
 	xopen* pa. intros D. xapp*. xmatch.
 	{ xchange* PArray_Desc_eq_Base. intros L' E.
-		inverts* Rpas as; tryifalse. intros Hpa E'.
+		inverts* Rpas as; tryifalse. intros Hpa E' Hub.
 		rewrite E in E'. inverts* E'.
 		xapp*. intros q. xsimpl*.
 		xchange* PArray_Base_close.
 		xchange* hforall_specialize.
-		xchange* hwand_hpure_l.
-		rewrites* <- E. rew_map*. xsimpl*. }
+		xchange* hwand_hpure_l; rewrites* <- E.
+		rewrites* <- PArray_Rec_eq. rew_map*. xsimpl*. }
 	{ xchange* PArray_Desc_eq_Diff. intros E.
-		inverts Rpas as; tryifalse. intros q Hpa E' Rq Hi.
+		inverts Rpas as; tryifalse. intros q Hpa E' Rq Hi Hdist.
 		rewrite E in E'. inverts* E'.
 		xchange* <- PArray_Desc_eq_Diff. xclose* pa.
 		xchange* hforall_specialize.
-		rewrites* E. rewrites* Points_into_eq_Diff.
 		xchange* hwand_hpure_l.
-		{ applys* IsPArray_inv_indom. }
-		{ rewrites* <- E. rew_map*.
-			xapp* IH; try math. intros a. xapp*. xvals*. } }
+		{ rewrites* (>> Points_into_eq_of_eq_Diff (M[pa])). applys* IsPArray_inv_indom. }
+		{ rew_map*. xapp* IH; try math. intros a. xapp*. xvals*. } }
 Qed.
 
 Hint Extern 1 (RegisterSpec parray_base_copy) => Provide parray_base_copy_spec.
@@ -572,23 +644,22 @@ Lemma parray_rebase_and_get_array_spec : forall A (IA: Inhab A) (EA: Enc A) (M: 
 	SPEC (parray_rebase_and_get_array pa)
 		PRE (Shared M)
 		POST (fun a =>
-			pa ~~~> `{ data' := (PArray_Base (B_ := A)) a } \*
+			pa ~~~> `{ data' := (PArray_Base (B_ := A)) a; maxdist' := maxdist (M[pa]) } \*
 			a ~> Array L \*
 			Group (PArray (A := A)) (M \-- pa) \*
 			\[Inv M]).
 Proof using.
-	introv Rpa. xcf*. xpay_skip.
+	introv Rpa. xcf*. xpay_fake.
 	xchange* Shared_eq. intros I. xchange* Group_rem.
 	xopen* pa. intros D. xapp*. xmatch.
 	{ xvals*. xchange* PArray_Desc_eq_Base. intros L' E'.
-		xsimpl*. inverts Rpa as.
-		{ intros Hpa E. rewrites* E in E'. inverts* E'. }
-		{ tryifalse. (* Ça ne fonctionne pas directement wtf *) } }
+		xsimpl*. inverts Rpa as; tryifalse.
+		intros Hpa E Hdist. applys* Memory_eq_inv_Base. }
 	{ xclose* pa. xchange* Group_add_again. rew_map*. xchange* <- Shared_eq.
 		xapp*. intros a.
-		xchange* Shared_eq. intros _. xchange* (>> Group_rem pa).
+		xchange* Shared_eq. intros _. xchange* Group_rem pa M.
 		xopen* pa. intros D. xapp*. xvals*. }
-Unshelve. auto. Qed.
+Qed.
 
 Hint Extern 1 (RegisterSpec parray_rebase_and_get_array) => Provide parray_rebase_and_get_array_spec.
 
@@ -600,14 +671,15 @@ Lemma parray_get_spec : forall A (IA: Inhab A) (EA: Enc A) (M: Memory A) (pa: pa
 		PRE \[]
 		POST (fun M' x => \[x = L[i]]).
 Proof using.
-	introv Rpa Hind. xcf*. simpl. xpay_skip.
-	xapp*. intros a Points. xapp*.
+	introv Rpa Hind. xcf*. simpl. xpay_fake.
+	xapp*. intros a I. xapp*.
 	xchange* PArray_Base_close.
 	xchange* Group_add_again.
 	xchanges* <- Shared_eq.
-	constructors*.
-	{ rew_map*. rewrites* <- dom_of_union_single_eq.
-		applys* Points_into_forall_update. applys* Inv_closure. }
+	{ constructors*.
+		{ rew_map*. rewrites* <- dom_of_union_single_eq.
+			applys* Points_into_forall_update. applys* Inv_closure. } }
+	{ applys* Extend_update_Base; simpl; auto. applys* IsPArray_inv_maxdist. }
 Qed.
 
 Hint Extern 1 (RegisterSpec parray_get) => Provide parray_get_spec.
@@ -620,37 +692,51 @@ Lemma parray_set_spec : forall A (IA: Inhab A) (EA: Enc A) (M: Memory A) (pa: pa
 		PRE \[]
 		POST (fun M' q => \[IsPArray M' (L[i := x]) q]).
 Proof using.
-	introv Rpa Hi. xcf*. simpl. xpay_skip.
-	xapp*. intros a Points. xapp*. xapp*.
-	xapp*. intros pb.
-	xapp*. xval*.
-	xchange* PArray_Diff_close. xchange* PArray_Base_close.
-	xchange* (heapdata pa pb). intros Diff.
-	xchange* Group_add_fresh. intros Hpb.
-	rewrites* update_remove_one_neq.
-	xchange* Group_add_again.
-	{ forwards*: IsPArray_inv_indom. }
-	{ assert (HMpb: Extend M (M[pb := Desc_Base L[i := x]])).
-		{ applys* Extend_add_fresh.
-			(* 3 lignes suivantes automatisable ? *)
-			rewrites* (>> eq_union_single_remove_one (dom M)).
-			intros* [|]; auto.
-			rewrites* dom_remove in Hpb. }
+	introv Rpa Hi. xcf*. simpl. xpay_fake.
+	xapp*. intros a I. xapp*. xapp*.
+	xif; intros x2.
+	{ xapp*. intros b. xapp*. xapp*. intros pb.
+		do 2 xchange* PArray_Base_close.
+		xchange* Group_add_again pa.
+		xchange* Group_add_fresh. intros Hpb.
 		xchanges* <- Shared_eq.
 		{ constructors*.
-			{ rew_map*. applys* Points_into_forall_update.
-				{ applys* Points_into_forall_update.
-					applys* Points_into_forall_subset (dom M).
-					{ rew_set. intros. rew_set. auto. (* automatisable ? *) }
-					{ applys* Inv_closure. } }
-				{ rewrites* Points_into_eq_Diff.
-					rew_set. auto. (* rew_set* ? *) } } }
+			{ rew_map*.
+				do 2 applys* Points_into_forall_update.
+				applys* Points_into_forall_subset (dom M).
+				applys* Inv_closure. } }
 		{ applys* Extend_trans.
-			applys* Extend_update_Diff pa (L[i := x]).
-				{ applys* index_update. }
-				{ rew_list. (* ne fait rien ? *) rewrites* update_update_same. rewrites* LibListZ.update_same. }
-				{ rew_map*. } }
-		{ applys* IsPArray_Base. rewrites* read_update_neq. rew_map*. } }
+			applys* Extend_update_Base; simpl; auto.
+			applys* IsPArray_inv_maxdist. }
+		{ applys* IsPArray_Base; rew_map*.
+			simpl. auto. } }
+	{ xapp*. xapp*. xapp*. xapp*. intros pb. xapp*. xval*.
+		xchange* PArray_Diff_close. xchange* PArray_Base_close.
+		xchange* (heapdata pa pb). intros Diff.
+		xchange* Group_add_fresh. intros Hpb.
+		rewrites* update_remove_one_neq.
+		xchange* Group_add_again.
+		{ forwards*: IsPArray_inv_indom pa. }
+		{ assert (HMpb: Extend M (M[pb := {| desc := Desc_Base L[i := x]; maxdist := maxdist (M[pa]) + 1 |}])).
+			{ applys* Extend_add_fresh.
+				(* 3 lignes suivantes automatisable ? *)
+				rewrites* (>> eq_union_single_remove_one (dom M)).
+				intros* [|]; auto.
+				rewrites* dom_remove in Hpb. }
+			xchanges* <- Shared_eq.
+			{ constructors*.
+				{ rew_map*. applys* Points_into_forall_update.
+					{ applys* Points_into_forall_update.
+						applys* Points_into_forall_subset (dom M).
+						applys* Inv_closure. }
+					{ rewrites* Points_into_eq_Diff. set_prove. } } }
+			{ applys* Extend_trans.
+				applys* Extend_update_Diff pa (L[i := x]) i (L[i]); rew_map*; simpl; auto.
+					{ applys* index_update. }
+					{ rewrites* update_update_same. rewrites* LibListZ.update_same. }
+					{ applys* IsPArray_Base; rew_map*.
+						simpl. rewrites* length_update. (* math *)skip. } }
+			{ applys* IsPArray_Base; rewrites* read_update_neq; rew_map*. simpl. (* math *) skip. } } }
 Qed.
 
 Hint Extern 1 (RegisterSpec parray_set) => Provide parray_set_spec.
@@ -662,11 +748,11 @@ Lemma parray_copy_spec : forall A (IA: Inhab A) (EA: Enc A) (M: Memory A) (pa: p
 		PRE \[]
 		POST (fun M' q => \[IsPArray M' L q]).
 Proof using.
-	introv Rpa. xcf*. simpl. xpay_skip.
+	introv Rpa. xcf*. simpl. xpay_fake.
 	xapp*. intros a. xapp*. intros q.
 	xchange* PArray_Base_close.
-	xchanges* Shared_add_fresh_Base; intros Hdom.
-	{ applys* IsPArray_Base. rew_map*. }
+	xchanges* Shared_add_fresh_Base L; intros Hdom.
+	applys* IsPArray_Base; rew_map*. simpl. auto.
 Qed.
 
 Hint Extern 1 (RegisterSpec parray_copy) => Provide parray_copy_spec.
